examples/ghc/theories/Base.v
@@ -1,22 +1,109 @@
+
+(* Disable notation conflict warnings *)
+Set Warnings "-notation-overridden".
+
+From Coq Require Import ssreflect ssrbool ssrfun.
+
 Require Import GHC.Base.
 Require Import GHC.Nat.
 Require Import Proofs.GHC.Base.
 Require Import Proofs.GHC.List.
+Require Import Proofs.Data.Foldable.
+Require Import Proofs.GhcTactics.
 
 Require Import Coq.Lists.List.
-
-Require Import Proofs.GhcTactics.
+Require Import Coq.Classes.RelationClasses.
+Require Import Coq.Classes.Morphisms.
+Require Import SetoidList.
 
 Import ListNotations.
 
 Open Scope Z_scope.
 
+
 Set Bullet Behavior "Strict Subproofs".
+
+(* I would love to be able to use rewriting instead of this 
+   lemma to do this. Why doesn't it work??? *)
+Lemma eq_replace_r : forall {a}`{EqLaws a}  (v1 v2 v3 : a),
+    (v2 == v3) -> (v1 == v2) = (v1 == v3).
+Proof.
+  intros.
+  rewrite -> H1. (* why does the ssreflect rewriting tactic not work here. *)
+  reflexivity.
+Qed.
+
+Lemma eq_replace_l : forall {a}`{EqLaws a} (v1 v2 v3 : a),
+    (v2 == v3) -> (v2 == v1) = (v3 == v1).
+Proof.
+  intros.
+  eapply Eq_m.
+  eauto.
+  eapply Eq_refl.
+Qed.
+
+
+(* Some cargo culting here. I'm not sure if we need to do all of this.*)
+
+Local Lemma parametric_eq_trans : forall (a : Type) (H : Eq_ a),
+  EqLaws a -> Transitive (fun x y : a => x == y).
+Proof.
+  intros.
+  intros x y z.
+  pose (k := Eq_trans).
+  eapply k.
+Defined. 
+
+Local Lemma parametric_eq_sym : forall (a : Type) (H : Eq_ a),
+  EqLaws a -> Symmetric (fun x y : a => x == y).
+Proof.
+  intros.
+  intros x y.
+  rewrite Eq_sym.
+  auto.
+Defined. 
+
+
+Add Parametric Relation {a}`{H: EqLaws a} : a 
+  (fun x y => x == y) 
+    reflexivity proved by Eq_refl 
+    symmetry proved by (@parametric_eq_sym a _ H)
+    transitivity proved by (@parametric_eq_trans a _ H) as parametric_eq.
+
+Instance: RewriteRelation (fun x y => x == y).
+
+
+Lemma eqlist_Foldable_elem : forall a (s s' : list a) `{EqLaws a}, 
+      eqlistA (fun x y => x == y) s s' ->
+      (forall a, Foldable.elem a s = Foldable.elem a s').
+Proof.
+  intros a s s' EQ EQL. intro H. induction H.
+  intro x.
+  rewrite elem_nil. auto.
+  intro y. 
+  repeat rewrite -> elem_cons.
+  rewrite IHeqlistA.
+  erewrite eq_replace_r; eauto.
+Qed.
+
 
 (**
 Some of this can migrate to [base-thy] at some point, but maybe some lemmas or
 tactics are rather specific.
 *)
+
+Lemma elem_eq : forall {A:Type}`{EqLaws A} (xs : list A) (a b : A),
+    a == b -> Foldable.elem a xs = Foldable.elem b xs.
+Proof.
+  move => A ??.
+  elim => // x xs IH.
+  move => a b h.
+  hs_simpl.
+  rewrite (IH _ _ h).
+  erewrite eq_replace_l; eauto.
+Qed.
+
+
 
 Lemma forallb_imp:
   forall a P Q (xs : list a),
